specs/lemmas/Spec.Blake2.Lemmas.fsti
@@ -6,6 +6,12 @@ open Spec.Hash.Definitions
 open Spec.Agile.Hash
 open FStar.Mul
 
+val lemma_blake2_hash_equivalence
+  (a:hash_alg{is_blake a}) (d:bytes{Seq.length d <= max_input_length a})
+  : Lemma
+    (Spec.Blake2.blake2 (to_blake_alg a) d 0 Seq.empty (Spec.Blake2.max_output (to_blake_alg a)) ==
+     Spec.Agile.Hash.hash a d)
+
 noextract inline_for_extraction
 val add_extra_i (a:hash_alg{is_blake a}) (ev:extra_state a) (i:U32.t) : extra_state a
 
